Pre-aristotle stuff

VCVio/OracleComp/SimSemantics/SimulateQ.lean
@@ -17,12 +17,7 @@ universe u v w
 
 variable {α β γ : Type u}
 
--- class HasSimulateQuery {ι} (spec : OracleSpec ι) (r : Type u → Type _)
---     (m : outParam (Type u → Type v)) [Monad m] [MonadLiftT (OracleQuery spec) m]
---     (n : outParam (Type u → Type w)) [Monad n] [MonadLiftT r n] where
---   simulateQ (impl : QueryImpl spec r) {α : Type u}
-
-/-- `HasSimulateQ spec r m n` means that an implementation of `OracleQuery spec` in terms of
+/- `HasSimulateQ spec r m n` means that an implementation of `OracleQuery spec` in terms of
 a computation in `r` results in a implementation of computations in `m` in terms of `n`.
 This implementation is given by a bundled monad hom `simulateQ`. We also require that queries
 can be lifted into `m`, and that `simulateQ` behaves naturally with this lift.
@@ -32,124 +27,132 @@ queries to `spec` in `r` and recursively substitutes that implementation in an `
 computation, to get a value in the new spec `r`.
 For example taking `r` to be `PMF` lets you asign output distributions to queries and
 get an output distribution for the whole computaiton. -/
-class HasSimulateQ {ι} (spec : OracleSpec ι) (r : Type u → Type*)
-    (m : (Type u → Type v)) [Monad m] [MonadLiftT (OracleQuery spec) m]
-    (n : outParam (Type u → Type w)) [Monad n] [MonadLiftT r n] where
-  /-- The mapping from `m` to `n` induced by implementing `spec` in terms of `r`. -/
-  simulateQ (impl : QueryImpl spec r) {α : Type u} : m α → n α
-  /-- `simulateQ` respects the underyling `pure` operation. -/
-  simulateQ_pure (impl : QueryImpl spec r) {α : Type u} (x : α) :
-      simulateQ impl (pure x : m α) = (pure x : n α)
-  /-- `simulateQ` respects the underlying `bind` operation. -/
-  simulateQ_bind (impl : QueryImpl spec r) {α β : Type u} (mx : m α) (my : α → m β) :
-      simulateQ impl (mx >>= my) = simulateQ impl mx >>= fun x => simulateQ impl (my x)
-  /-- Simulating a query is the same as applying the implementation to the query input. -/
-  simulateQ_liftM (impl : QueryImpl spec r) {α : Type u} (q : OracleQuery spec α) :
-    (simulateQ impl) (liftM q : m α) = q.cont <$> liftM (impl q.input)
+-- class HasSimulateQ {ι} (spec : OracleSpec ι) (r : Type u → Type*)
+--     (m : (Type u → Type v)) [Monad m] [MonadLiftT (OracleQuery spec) m]
+--     (n : outParam (Type u → Type w)) [Monad n] [MonadLiftT r n] where
+--   /-- The mapping from `m` to `n` induced by implementing `spec` in terms of `r`. -/
+--   simulateQ (impl : QueryImpl spec r) {α : Type u} : m α → n α
+--   /-- `simulateQ` respects the underyling `pure` operation. -/
+--   simulateQ_pure (impl : QueryImpl spec r) {α : Type u} (x : α) :
+--       simulateQ impl (pure x : m α) = (pure x : n α)
+--   /-- `simulateQ` respects the underlying `bind` operation. -/
+--   simulateQ_bind (impl : QueryImpl spec r) {α β : Type u} (mx : m α) (my : α → m β) :
+--       simulateQ impl (mx >>= my) = simulateQ impl mx >>= fun x => simulateQ impl (my x)
+--   /-- Simulating a query is the same as applying the implementation to the query input. -/
+--   simulateQ_liftM (impl : QueryImpl spec r) {α : Type u} (q : OracleQuery spec α) :
+--     (simulateQ impl) (liftM q : m α) = q.cont <$> liftM (impl q.input)
 
-export HasSimulateQ (simulateQ simulateQ_pure simulateQ_bind simulateQ_liftM)
+-- export HasSimulateQ (simulateQ simulateQ_pure simulateQ_bind simulateQ_liftM)
 
-attribute [simp, grind =] simulateQ_liftM simulateQ_pure simulateQ_bind
+-- attribute [simp, grind =] simulateQ_liftM simulateQ_pure simulateQ_bind
 
 section simulateQ
 
+/-- Given an implementation of `spec` in the monad `r`, convert an `OracleComp spec α` to a
+implementation in `r α` by substituting `impl t` for `query t` throughout. -/
+def simulateQ {ι} {spec : OracleSpec ι} {r : Type u → Type _} [Monad r]
+    (impl : QueryImpl spec r) {α : Type u} (mx : OracleComp spec α) : r α :=
+  PFunctor.FreeM.mapM impl mx
+
 variable {ι} {spec : OracleSpec ι} {r m n : Type u → Type*}
-    [Monad m] [MonadLiftT (OracleQuery spec) m] [Monad n]
-    [MonadLiftT r n] [HasSimulateQ spec r m n] (impl : QueryImpl spec r)
+    [Monad r] (impl : QueryImpl spec r)
+
+@[simp, grind =]
+lemma simulateQ_pure (x : α) :
+    simulateQ impl (pure x : OracleComp spec α) = pure x := rfl
+
+@[simp, grind =]
+lemma simulateQ_bind [LawfulMonad r] (mx : OracleComp spec α) (my : α → OracleComp spec β) :
+    simulateQ impl (mx >>= my) = simulateQ impl mx >>= fun x => simulateQ impl (my x) := by
+  simp [simulateQ]
 
 /-- Version of `simulateQ` that bundles into a monad hom. -/
 @[reducible]
-def simulateQ' (impl : QueryImpl spec r) : m →ᵐ n where
+def simulateQ' [LawfulMonad r] (impl : QueryImpl spec r) : OracleComp spec →ᵐ r where
   toFun {_α} mx := simulateQ impl mx
   toFun_pure' _ := simulateQ_pure _ _
   toFun_bind' _ _ := simulateQ_bind _ _ _
 
-def simulateQ'' {ι} {spec : OracleSpec ι} {r m n : Type u → Type*}
-    [Monad m] [MonadLiftT (OracleQuery spec) m] [Monad n]
-    [MonadLiftT r n] [HasSimulateQ spec r m n]
-    (impl : QueryImpl spec r) {α : Type u} (mx : m α) : n α :=
-  simulateQ impl mx
-
 @[simp, grind =]
-lemma simulateQ_query [LawfulMonad n] (t : spec.Domain) :
-    simulateQ impl (query t : m (spec.Range t)) = liftM (impl t) := by
-  simp [query_def, HasSimulateQ.simulateQ_liftM (m := m)]
+lemma simulateQ_query [LawfulMonad r] (q : OracleQuery spec α) :
+    simulateQ impl (liftM q) = q.cont <$> (impl q.input) := by
+  simp [simulateQ, PFunctor.FreeM.mapM.eq_def]
 
 @[simp]
-lemma simulateQ_query_bind [LawfulMonad n] (t : spec.Domain) (ou : spec.Range t → m β) :
-    simulateQ impl ((query t : m _) >>= ou) =
-      liftM (impl t) >>= fun u => simulateQ impl (ou u) := by aesop
+lemma simulateQ_query_bind [LawfulMonad r] (q : OracleQuery spec α)
+    (ou : α → OracleComp spec β) : simulateQ impl (liftM q >>= ou) =
+      liftM (impl q.input) >>= fun u => simulateQ impl (ou (q.cont u)) := by aesop
 
 @[simp, grind =]
-lemma simulateQ_map [LawfulMonad m] [LawfulMonad n] (mx : m α) (f : α → β) :
+lemma simulateQ_map [LawfulMonad r] (mx : OracleComp spec α) (f : α → β) :
     simulateQ impl (f <$> mx) = f <$> simulateQ impl mx := by
   simp [map_eq_bind_pure_comp]
 
 @[simp]
-lemma simulateQ_seq [LawfulMonad m] [LawfulMonad n] (og : m (α → β)) (mx : m α) :
+lemma simulateQ_seq [LawfulMonad r] (og : OracleComp spec (α → β)) (mx : OracleComp spec α) :
     simulateQ impl (og <*> mx) = simulateQ impl og <*> simulateQ impl mx := by
   simp [seq_eq_bind_map]
 
 @[simp]
-lemma simulateQ_seqLeft [LawfulMonad m] [LawfulMonad n] (mx : m α) (my : m β) :
+lemma simulateQ_seqLeft [LawfulMonad r] (mx : OracleComp spec α) (my : OracleComp spec β) :
     simulateQ impl (mx <* my) = simulateQ impl mx <* simulateQ impl my := by
   simp [seqLeft_eq_bind]
 
 @[simp]
-lemma simulateQ_seqRight [LawfulMonad m] [LawfulMonad n] (mx : m α) (my : m β) :
+lemma simulateQ_seqRight [LawfulMonad r] (mx : OracleComp spec α) (my : OracleComp spec β) :
     simulateQ impl (mx *> my) = simulateQ impl mx *> simulateQ impl my := by
   simp [seqRight_eq_bind]
 
 @[simp]
-lemma simulateQ_ite (p : Prop) [Decidable p] (mx mx' : m α) :
+lemma simulateQ_ite (p : Prop) [Decidable p] (mx mx' : OracleComp spec α) :
     simulateQ impl (ite p mx mx') = ite p (simulateQ impl mx) (simulateQ impl mx') := by
   split_ifs <;> rfl
 
 end simulateQ
 
-namespace OracleQuery
+-- namespace OracleQuery
 
-variable {ι} {ι'} {spec : OracleSpec ι} {spec' : OracleSpec ι'}
+-- variable {ι} {ι'} {spec : OracleSpec ι} {spec' : OracleSpec ι'}
 
-/-- Given a map from queries in `spec` to queries in `spec'`, lift to a map on `OracleComp`
-by substituting each query for the new implementation in `spec'`. -/
-instance {ι} {ι'} {spec : OracleSpec ι} {spec' : OracleSpec ι'} :
-    HasSimulateQ spec (OracleQuery spec') (OracleComp spec) (OracleComp spec') where
-  simulateQ impl α mx := PFunctor.FreeM.mapM (QueryImpl.liftTarget _ impl) mx
-  simulateQ_pure _ _ _ := by simp
-  simulateQ_bind _ _ _ _ := by simp
-  simulateQ_liftM _ _ _ := rfl
+-- /-- Given a map from queries in `spec` to queries in `spec'`, lift to a map on `OracleComp`
+-- by substituting each query for the new implementation in `spec'`. -/
+-- instance {ι} {ι'} {spec : OracleSpec ι} {spec' : OracleSpec ι'} :
+--     HasSimulateQ spec (OracleQuery spec') (OracleComp spec) (OracleComp spec') where
+--   simulateQ impl α mx := PFunctor.FreeM.mapM (QueryImpl.liftTarget _ impl) mx
+--   simulateQ_pure _ _ _ := by simp
+--   simulateQ_bind _ _ _ _ := by simp
+--   simulateQ_liftM _ _ _ := rfl
 
-@[grind =]
-lemma simulateQ_def (impl : QueryImpl spec (OracleQuery spec'))
-    (mx : OracleComp spec α) : (simulateQ impl mx) =
-    PFunctor.FreeM.mapMHom (fun x => liftM (impl x)) mx := rfl
+-- @[grind =]
+-- lemma simulateQ_def (impl : QueryImpl spec (OracleQuery spec'))
+--     (mx : OracleComp spec α) : (simulateQ impl mx) =
+--     PFunctor.FreeM.mapMHom (fun x => liftM (impl x)) mx := rfl
 
-/-- `QueryImpl.id` is an identity for `simulateQ` with implementaiton in `OracleQuery spec`. -/
-@[simp] lemma simulateQ_id (mx : OracleComp spec α) :
-    simulateQ (QueryImpl.id spec) mx = mx := by
-  induction mx using OracleComp.inductionOn with
-  | pure x => simp
-  | query_bind t mx h => simp [h]
+-- /-- `QueryImpl.id` is an identity for `simulateQ` with implementaiton in `OracleQuery spec`. -/
+-- @[simp] lemma simulateQ_id (mx : OracleComp spec α) :
+--     simulateQ (QueryImpl.id spec) mx = mx := by
+--   induction mx using OracleComp.inductionOn with
+--   | pure x => simp
+--   | query_bind t mx h => simp [h]
 
-/-- Lifting queries to their original implementation has no effect on a computation. -/
-lemma simulateQ_ofLift_eq_self {α} (mx : OracleComp spec α) :
-    simulateQ (QueryImpl.ofLift spec (OracleQuery spec)) mx = mx := by simp
+-- /-- Lifting queries to their original implementation has no effect on a computation. -/
+-- lemma simulateQ_ofLift_eq_self {α} (mx : OracleComp spec α) :
+--     simulateQ (QueryImpl.ofLift spec (OracleQuery spec)) mx = mx := by simp
 
-end OracleQuery
+-- end OracleQuery
 
-namespace OracleComp
+-- namespace OracleComp
 
-/-- Given a `QueryImpl` of `spec` in terms of `n` we map any computation in
-`OracleComp spec` to `n` by replacing queries with the corresponding implementation.
-Taking `n` to be `PMF`, `Set`, etc. makes it possible to substitute each query for some denotation
-like an output distribution and get the corresponding value for the entire computation.  -/
-instance {ι} {spec : OracleSpec ι} {n : Type u → Type w} [Monad n] [LawfulMonad n] :
-    HasSimulateQ spec n (OracleComp spec) n where
-  simulateQ impl {α} mx := PFunctor.FreeM.mapM impl mx
-  simulateQ_pure _ _ := by simp
-  simulateQ_bind _ _ _ := by simp
-  simulateQ_liftM _ _ := by simp [PFunctor.FreeM.mapM]
+-- /-- Given a `QueryImpl` of `spec` in terms of `n` we map any computation in
+-- `OracleComp spec` to `n` by replacing queries with the corresponding implementation.
+-- Taking `n` to be `PMF`, `Set`, etc. makes it possible to substitute each query for some denotation
+-- like an output distribution and get the corresponding value for the entire computation.  -/
+-- instance {ι} {spec : OracleSpec ι} {n : Type u → Type w} [Monad n] [LawfulMonad n] :
+--     HasSimulateQ spec n (OracleComp spec) n where
+--   simulateQ impl {α} mx := PFunctor.FreeM.mapM impl mx
+--   simulateQ_pure _ _ := by simp
+--   simulateQ_bind _ _ _ := by simp
+--   simulateQ_liftM _ _ := by simp [PFunctor.FreeM.mapM]
 
 variable {ι} {spec : OracleSpec ι} {n : Type u → Type v}
   [Monad n] [LawfulMonad n] (impl : QueryImpl spec n)
@@ -169,50 +172,50 @@ lemma simulateQ_id' (mx : OracleComp spec α) :
 lemma simulateQ_ofLift_eq_self {α} (mx : OracleComp spec α) :
     simulateQ (QueryImpl.ofLift spec (OracleComp spec)) mx = mx := by simp
 
-end OracleComp
+-- end OracleComp
 
-section OptionT
+-- section OptionT
 
-variable {ι} {spec : OracleSpec ι} {r m n : Type u → Type*}
+-- variable {ι} {spec : OracleSpec ι} {r m n : Type u → Type*}
 
-/-- Apply `simulateQ` "underneath" an `OptionT` transformer. -/
-instance [Monad m] [MonadLiftT (OracleQuery spec) m]
-    [Monad n] [LawfulMonad n] [MonadLiftT r n]
-    [HasSimulateQ spec r m n] : HasSimulateQ spec r (OptionT m) (OptionT n) where
-  simulateQ impl α mx := OptionT.mk (simulateQ impl (OptionT.run mx))
-  simulateQ_pure := sorry
-  simulateQ_bind := sorry
-    -- have : m →ᵐ n := simulateQ impl
-    -- refine OptionT.mapM' ?_
-    -- refine MonadHom.comp ?_ this
-    -- refine MonadHom.ofLift n (OptionT n)
-  simulateQ_liftM impl α q := by
-    stop
-    refine OptionT.ext ?_
-    simp
-    have : (liftM q : OptionT m α) = OptionT.lift (liftM q) := rfl
-    simp [OptionT.mapM']
-    simp [OptionT.run]
-    rw [this]
-    simp [OptionT.lift, OptionT.mk]
-    simp only [map_eq_bind_pure_comp, Function.comp_def]
-    rfl
+-- /-- Apply `simulateQ` "underneath" an `OptionT` transformer. -/
+-- instance [Monad m] [MonadLiftT (OracleQuery spec) m]
+--     [Monad n] [LawfulMonad n] [MonadLiftT r n]
+--     [HasSimulateQ spec r m n] : HasSimulateQ spec r (OptionT m) (OptionT n) where
+--   simulateQ impl α mx := OptionT.mk (simulateQ impl (OptionT.run mx))
+--   simulateQ_pure := sorry
+--   simulateQ_bind := sorry
+--     -- have : m →ᵐ n := simulateQ impl
+--     -- refine OptionT.mapM' ?_
+--     -- refine MonadHom.comp ?_ this
+--     -- refine MonadHom.ofLift n (OptionT n)
+--   simulateQ_liftM impl α q := by
+--     stop
+--     refine OptionT.ext ?_
+--     simp
+--     have : (liftM q : OptionT m α) = OptionT.lift (liftM q) := rfl
+--     simp [OptionT.mapM']
+--     simp [OptionT.run]
+--     rw [this]
+--     simp [OptionT.lift, OptionT.mk]
+--     simp only [map_eq_bind_pure_comp, Function.comp_def]
+--     rfl
 
--- lemma simulateQ_def
+-- -- lemma simulateQ_def
 
-@[simp, grind =]
-lemma simulateQ_id' (mx : OptionT (OracleComp spec) α) :
-    simulateQ (QueryImpl.id' spec) mx = mx := by
+-- @[simp, grind =]
+-- lemma simulateQ_id' (mx : OptionT (OracleComp spec) α) :
+--     simulateQ (QueryImpl.id' spec) mx = mx := by
 
-  sorry
+--   sorry
 
-end OptionT
+-- end OptionT
 
-section ErrorT
+-- section ErrorT
 
--- TODO
+-- -- TODO
 
-end ErrorT
+-- end ErrorT
 
 section tests
 
